more work on multistep Hoare, changing approach to not assume termination

Semantics/Gensyn_Sem_Small.thy
@@ -1,14 +1,29 @@
 theory Gensyn_Sem_Small imports "../Gensyn" "../Gensyn_Descend" "../Mergeable/Mergeable"
+                                
 
 begin
+
+datatype gensyn_small_error =
+  Ok
+  | BadPath
+  | NoFuel
+  | Halted (* this means we executed _past_ the end *)
+
 
 record ('x, 'mstate) g_semr =
   gsr_rel :: "'x \<Rightarrow> 'mstate \<Rightarrow> 'mstate \<Rightarrow> bool"
   gsr_getpath :: "'mstate \<Rightarrow> childpath \<Rightarrow> bool"
+  gsr_getdir :: "'mstate \<Rightarrow> dir \<Rightarrow> bool"
 
 record ('x, 'mstate) g_sem =
   gs_sem :: "'x \<Rightarrow> 'mstate \<Rightarrow> 'mstate"
   gs_getpath :: "'mstate \<Rightarrow> childpath option"
+  gs_getdir :: "'mstate \<Rightarrow> dir"
+
+fun gs_halted :: "('x, 'mstate) g_sem \<Rightarrow> 'mstate \<Rightarrow> bool" where
+"gs_halted gs m = (gs_getpath gs m = None)"
+
+(* gs_getflag :: "'mstate \<Rightarrow> gensyn_small_flag" *)
 
 definition gensyn_sem_small ::
   "('x, 'mstate) g_semr \<Rightarrow> 
@@ -18,6 +33,7 @@ definition gensyn_sem_small ::
  (\<exists> x l . gensyn_get syn cp = Some (G x l) \<and>
   gsr_rel gsr x m m'))"
 
+(*
 inductive gensyn_sem_small_many ::
   "('x, 'mstate) g_semr \<Rightarrow> 
    'x gensyn \<Rightarrow> 'mstate \<Rightarrow> 'mstate \<Rightarrow> bool" where
@@ -33,38 +49,56 @@ definition gensyn_sem_small_many_halt ::
 "gensyn_sem_small_many_halt gsr syn m m' =
  (gensyn_sem_small_many gsr syn m m' \<and>
  (\<forall> cp . \<not> gsr_getpath gsr m' cp))"
-
-datatype gensyn_small_flag =
-  Exec
-  | Halt
-  | BadPath
-  | NoFuel
+*)
 
 fun gensyn_sem_small_exec ::
   "('x, 'mstate) g_sem \<Rightarrow>
    'x gensyn \<Rightarrow>
    'mstate \<Rightarrow>
-   ('mstate * gensyn_small_flag)" where
+   ('mstate * gensyn_small_error)" where
 "gensyn_sem_small_exec gs syn m =
  (case gs_getpath gs m of
-  None \<Rightarrow> (m, Halt)
+  None \<Rightarrow> (m, Ok)
   | Some cp \<Rightarrow> 
     (case gensyn_get syn cp of
      None \<Rightarrow> (m, BadPath)
-     | Some (G x _) \<Rightarrow> (gs_sem gs x m, Exec)))"
+     | Some (G x _) \<Rightarrow> (gs_sem gs x m, Ok)))"
 
+(*
 fun gensyn_sem_small_exec_many ::
   "('x, 'mstate) g_sem \<Rightarrow>
    'x gensyn \<Rightarrow>
    nat \<Rightarrow>
    'mstate \<Rightarrow>
-   ('mstate * gensyn_small_flag)" where
+   ('mstate * gensyn_small_error)" where
 "gensyn_sem_small_exec_many gs syn 0 m =
-  (m, NoFuel)"
+  (case gs_getpath gs m of
+    None \<Rightarrow> (m, Ok)
+    | _ \<Rightarrow>  (m, NoFuel))"
 | "gensyn_sem_small_exec_many gs syn (Suc n) m =
-   (case gensyn_sem_small_exec gs syn m of
-    (m', Exec) \<Rightarrow> gensyn_sem_small_exec_many gs syn n m'
-    | (m', f) \<Rightarrow> (m', f))"
+   (case gs_getpath gs m of
+    None \<Rightarrow> (m, Halted)
+    | _ \<Rightarrow> (case gensyn_sem_small_exec gs syn m of
+            (m', Ok) \<Rightarrow> gensyn_sem_small_exec_many gs syn n m'
+            | (m', f) \<Rightarrow> (m', f)))"
+*)
+
+(* one approach: just don't keep out of fuel flag. *)
+fun gensyn_sem_small_exec_many ::
+  "('x, 'mstate) g_sem \<Rightarrow>
+   'x gensyn \<Rightarrow>
+   nat \<Rightarrow>
+   'mstate \<Rightarrow>
+   ('mstate * gensyn_small_error)" where
+"gensyn_sem_small_exec_many gs syn 0 m =
+  (m, Ok)"
+| "gensyn_sem_small_exec_many gs syn (Suc n) m =
+   (case gs_getpath gs m of
+    None \<Rightarrow> (m, Ok)
+    | _ \<Rightarrow> (case gensyn_sem_small_exec gs syn m of
+            (m', Ok) \<Rightarrow> gensyn_sem_small_exec_many gs syn n m'
+            | (m', f) \<Rightarrow> (m', f)))"
+
 (*
 fun gensyn_sem_small_exec_many ::
   "('x, 'mstate) g_sem \<Rightarrow>
@@ -80,18 +114,22 @@ fun gensyn_sem_small_exec_many ::
     | (m', f) \<Rightarrow> (m', f))"
 *)
 
+(* TODO: the ordering of checks is weird here and will lead to weird traces. *)
 fun gensyn_sem_small_exec_trace' ::
   "('x, 'mstate) g_sem \<Rightarrow>
    'x gensyn \<Rightarrow>
    nat \<Rightarrow>
    'mstate list \<Rightarrow>
    'mstate \<Rightarrow>
-   ('mstate list * gensyn_small_flag)" where
+   ('mstate list * gensyn_small_error)" where
 "gensyn_sem_small_exec_trace' gs syn 0 l m =
   (m#l, NoFuel)"
 | "gensyn_sem_small_exec_trace' gs syn (Suc n) l m =
    (case gensyn_sem_small_exec gs syn m of
-    (m', Exec) \<Rightarrow> gensyn_sem_small_exec_trace' gs syn n (m#l) m'
+    (m', Ok) \<Rightarrow> 
+      (case gs_getpath gs m of
+        None \<Rightarrow> (m'#m#l, Ok)
+        | _ \<Rightarrow> gensyn_sem_small_exec_trace' gs syn n (m#l) m')
     | (m', f) \<Rightarrow> (m'#m#l, f))"
 
 fun gensyn_sem_small_exec_trace ::
@@ -99,7 +137,7 @@ fun gensyn_sem_small_exec_trace ::
    'x gensyn \<Rightarrow>
    nat \<Rightarrow>
    'mstate \<Rightarrow>
-   ('mstate list * gensyn_small_flag)" where
+   ('mstate list * gensyn_small_error)" where
 "gensyn_sem_small_exec_trace gs syn n m =
  (case gensyn_sem_small_exec_trace' gs syn n [] m of
   (l, f) \<Rightarrow> (rev l, f))"
